\section{Aufgabe 1}
    \subsection{a)} 
        $$
        \lim_{n\to\infty} \frac{n^2}{n^3+1} = \lim_{n\to\infty} \frac{\frac{1}{n}}{1 + \frac{1}{n^3}} = \frac{\lim_{n \to \infty}\frac{1}{n}}{\lim_{n \to \infty}(1+\frac{1}{n^3})}=\frac{0}{1+0}=\frac{0}{1}=0
        $$

    \subsection{b)}
        $$
        \lim_{n \to \infty} \frac{(n+1)(4n^2-3)}{(3n-5)^3}=\lim_{n \to \infty} \frac{n(1+\frac{1}{n})n^2(4-\frac{3}{n^2})}{(n(3-\frac{5}{n}))^3}=\lim_{n \to \infty}\frac{n^3(1+\frac{1}{n})(4-\frac{3}{n^2})}{n^3(3-\frac{5}{n})^3}
        $$
        $$
        =\lim_{n \to \infty}\frac{(1+\frac{1}{n})(4-\frac{3}{n^2})}{(3-\frac{5}{n})^3} = \frac{\lim_{n \to \infty}(1+\frac{1}{n})(4-\frac{3}{n^2})}{\lim_{n \to \infty}(3-\frac{5}{n})^3}=\frac{1\cdot 4}{3^3} = \frac{4}{27}
        $$

    \subsection{c)}
        $$
        \lim_{n \to \infty}\sqrt{4n^2+3n}-2n=\lim_{n \to \infty}\frac{(\sqrt{4n^2+3n}-2n)(\sqrt{4n^2+3n}+2n)}{\sqrt{4n^2+3n}+2n}=\lim_{n \to \infty}\frac{3n}{\sqrt{4n^2+3n}+2n}=3\lim_{n \to \infty}\frac{n}{\sqrt{4n^2+3n}+2n}
        $$
        $$
        =3\lim_{n \to \infty}\frac{n}{\sqrt{n^2(4+\frac{3}{n})}+2n}=3\lim_{n \to \infty}\frac{n}{n\sqrt{(4+\frac{3}{n})}+2n}=3\lim_{n \to \infty}\frac{1}{\sqrt{(4+\frac{3}{n})}+2}=3\cdot\frac{1}{\lim_{n \to \infty}\sqrt{(4+\frac{3}{n})}+2}
        $$
        $$
        3\cdot \frac{1}{\sqrt{4}+2}=\frac{3}{4}
        $$

    \subsection{d)}
        $$
        \lim_{n \to \infty}\frac{\sqrt{n+a}-\sqrt{n}}{\sqrt{n+b}-\sqrt{n}}=\lim_{n \to \infty}\frac{\frac{a}{\sqrt{n+a}+\sqrt{n}}}{\frac{b}{\sqrt{n+b}+\sqrt{n}}} = \frac{a}{b} \lim_{n \to \infty}\frac{\frac{1}{\sqrt{n+a}+\sqrt{n}}}{\frac{1}{\sqrt{n+b}+\sqrt{n}}}
        $$
        Für $n \to \infty$ kann man annehmen: $\sqrt{n+a},\sqrt{n+b}\to \sqrt{n}\Rightarrow$ für $n \to \infty: \sqrt{n+a}+\sqrt{n}, \sqrt{n+b}+\sqrt{n} \to 2\sqrt{n}$
        $$\Rightarrow \text{für } n \to \infty \frac{a}{b} \lim_{n \to \infty}\frac{\frac{1}{\sqrt{n+a}+\sqrt{n}}}{\frac{1}{\sqrt{n+b}+\sqrt{n}}} \to \frac{a}{b} \lim_{n \to \infty}\frac{\frac{1}{2\sqrt{n}}}{\frac{1}{2\sqrt{n}}}=\frac{a}{b}\lim_{n \to \infty}1=\frac{a}{b}$$